done/Iron/Data/Bool.v
@@ -1,0 +1,28 @@
+
+
+Lemma beq_true_split
+ :  forall A B
+ ,  true = andb A B
+ -> true = A /\ true = B.
+Proof.
+ intros.
+ destruct A. 
+  tauto.
+  simpl in H. congruence.
+Qed.
+Hint Resolve beq_true_split.
+
+
+Lemma beq_false_split
+ :  forall A B
+ ,  false = andb A B
+ -> false = A \/ false = B.
+Proof.
+ intros.
+ destruct A.
+  simpl in H. subst. tauto.
+  tauto.
+Qed.
+Hint Resolve beq_false_split.
+
+
